rename P1_UInt32 into Impl.Test

test.c
@@ -1,4 +1,4 @@
-#include "P1_UInt32.c"
+#include "Impl_Test.c"
 #include <stdlib.h>
 #include <stdbool.h>
 
@@ -13,10 +13,10 @@ int main(int argc, char** argv) {
   }
   //printf("%s\n", argv[0]);
   uint64_t x = strtoull(argv[1], NULL, 0);
-  uint64_t* random_data = malloc(x * sizeof(uint64_t));
-  arc4random_buf(random_data, x * sizeof(uint64_t));
+  int64_t* random_data = malloc(x * sizeof(int64_t));
+  arc4random_buf(random_data, x * sizeof(int64_t));
   void* ptr = NULL;
-  uint64_t rd = 0;
+  int64_t rd = 0;
   uint64_t s = 0;
   puts("AVL implementation test.");
   puts("The supplied number of random values");
@@ -27,17 +27,17 @@ int main(int argc, char** argv) {
 
   for (size_t i = 0; i < x; i++) {
     rd = random_data[i];
-    //printf("rd=%lui\n", rd);
-    ptr = P1_UInt32_insert_avl(true, P1_UInt32_compare, ptr, rd);
+    //printf("rd=%li\n", rd);
+    ptr = Impl_Test_insert_avl(true, Impl_Test_compare, ptr, rd);
   }
-  s = P1_UInt32_sot_wds(ptr);
+  s = Impl_Test_sot_wds(ptr);
   puts("Should be equal to the supplied argument.");
   printf("s=%lui\n", s);
 
   //bool b = false;
   //for (size_t i = 0; i < x; i++) {
   //  rd = random_data[i];
-  //  b = P1_UInt32_member(P1_UInt32_compare, ptr, rd);
+  //  b = Impl_Test_member(Impl_Test_compare, ptr, rd);
   //  if (! b) {
   //    puts("Error: some element was not properly inserted.");
   //    return 1;
@@ -46,10 +46,10 @@ int main(int argc, char** argv) {
 
   //for (size_t i = 0; i < x; i++) {
   //  rd = random_data[i];
-  //  ptr = P1_UInt32_delete_avl(P1_UInt32_compare, ptr, rd);
+  //  ptr = Impl_Test_delete_avl(Impl_Test_compare, ptr, rd);
   //}
   //puts("Should be equal to zero.");
-  //s = P1_UInt32_sot_wds(ptr);
+  //s = Impl_Test_sot_wds(ptr);
   //printf("s=%lui\n", s);
 
   //uint64_t s1 = 0;
@@ -57,15 +57,15 @@ int main(int argc, char** argv) {
   //uint64_t r1 = 0;
   //uint64_t r2 = 0;
   //void* ptr = NULL;
-  //ptr = P1_UInt32_main5(x);
-  //s1 = P1_UInt32_sot_wds(ptr);
+  //ptr = Impl_Test_main5(x);
+  //s1 = Impl_Test_sot_wds(ptr);
   //printf("s1=%lui\n", s1);
-  //r1 = P1_UInt32_main6_aux(ptr, x, true);
+  //r1 = Impl_Test_main6_aux(ptr, x, true);
   //printf("r1=%lui\n", r1);
-  //ptr = P1_UInt32_main7_aux (ptr, x);
-  //s2 = P1_UInt32_sot_wds(ptr);
+  //ptr = Impl_Test_main7_aux (ptr, x);
+  //s2 = Impl_Test_sot_wds(ptr);
   //printf("s2=%lui\n", s2);
-  //r2 = P1_UInt32_main6_aux(ptr, x, false);
+  //r2 = Impl_Test_main6_aux(ptr, x, false);
   //printf("r2=%lui\n", r2);
   return 0;
 }
